Add Euler decomposition

Main.lean
@@ -132,6 +132,18 @@ example : ∃ d', exercise3point7 ≈z d' := by
   zx_unsp 20 ⟨0, 1⟩ ⟨1, 1⟩ [3]
   zx_rfl
 
+-- Hadamard decomposition test
+def hadWire : ZXDiagram :=
+  ZXDiagram.ofList
+    [.input 0, .hadamard, .output 0]
+    [⟨0, 1⟩, ⟨1, 2⟩]
+#html hadWire.toHtml
+
+example : ∃ d', hadWire ≈z d' := by
+  zx_explore
+  zx_eu 1 6
+  zx_rfl
+
 -- Current challenge: Graph equality
 --   Implemented some normalization - edges are always ordered, phases are always simplified
 --   Another cheap win - strip out nones from the node list
